Progress on quoting refinements

rupicola/refinements/QExp.fst
@@ -24,11 +24,31 @@ let extend (t:Type0) (g:env)
           else g (y-1)
 
 (** F* evaluation environment **)
-assume val fs_env (g:env) : Type u#0
-assume val fs_empty : fs_env empty
-assume val fs_stack : #g:env -> fsG:fs_env g -> #t:Type -> t -> fs_env (extend t g)
-assume val fs_hd : #g:env -> #t:Type -> fs_env (extend t g) -> t
-assume val fs_tail : #t:Type -> #g:env -> fs_env (extend t g) -> fs_env g
+module FE = FStar.FunctionalExtensionality
+
+type fs_env g =
+  FE.restricted_t (x:var{Some? (g x)}) (fun x -> Some?.v (g x))
+
+unfold
+val fs_hd : #g:_ -> #t:Type -> fs_env (extend t g) -> t
+let fs_hd  fsG = fsG 0
+
+unfold
+val fs_stack : #g:_ -> fsG:fs_env g -> #t:Type -> t -> fs_env (extend t g)
+let fs_stack #g fsG #t fs_v =
+  FE.on_dom
+    (x:var{Some? ((extend t g) x)})
+    #(fun x -> (Some?.v ((extend t g) x)))
+    (fun y ->
+      if y = 0 then fs_v else fsG (y-1))
+
+unfold
+val fs_tail : #t:Type -> #g:_ -> fs_env (extend t g) -> fs_env g
+let fs_tail #t #g fsG =
+  FE.on_dom
+    (x:var{Some? (g x)})
+    #(fun x -> Some?.v (g x))
+    (fun y -> fsG (y+1))
 
 type spec_env (g:env) (a:Type) =
   fsG:fs_env g -> pure_wp a
@@ -150,6 +170,62 @@ val helper_lambda : #g :env ->
 let helper_lambda #g #a f =
   fun fsG -> f (fs_tail #a fsG) (fs_hd fsG)
 
+val wp_lambda0' :
+  #g :env ->
+  #a :Type u#0 ->
+  #b :Type u#b ->
+  wpCtx : spec_env (extend a g) b ->
+  wpFun : (a -> pure_wp b) ->
+  fs_oexp (extend a g) b wpCtx ->
+  fsG:fs_env g ->
+  pure_wp' (x:a -> PURE b (wpFun x))
+
+let wp_lambda0' #g #a #b wpCtx wpFun body fsG =
+  fun (p:pure_post (x:a -> PURE b (wpFun x))) ->
+    (forall (x: a) (p: pure_post b).
+      wpFun x p ==>
+      (wpCtx (fs_stack fsG x) (fun _ -> True) /\ (** Cezar: this is the only extra thing compared to the VC created by F* **)
+      wpCtx (fs_stack fsG x) (fun res ->
+        res == body (fs_stack fsG x) ==>
+        pure_return _ res p))
+    //) /\ pure_return _ (fun x -> body (fs_stack fsG x)) p // Cezar: this is not accepted?
+    ) /\ p (fun x -> body (fs_stack fsG x))
+
+let lem_wp_lambda'_monotonic #g #a #b wpCtx wpFun body fsG : Lemma (pure_wp_monotonic0 (x:a -> PURE b (wpFun x)) (wp_lambda0' #g #a #b wpCtx wpFun body fsG)) =
+  admit ()
+
+val wp_lambda' :
+  #g :env ->
+  #a :Type u#0 ->
+  #b :Type u#b ->
+  wpCtx : spec_env (extend a g) b ->
+  wpFun : (a -> pure_wp b) ->
+  fs_oexp (extend a g) b wpCtx ->
+  fsG:fs_env g ->
+  pure_wp (x:a -> PURE b (wpFun x))
+let wp_lambda' #g (#a:Type u#0) (#b:Type u#b) wpCtx wpFun body fsG : pure_wp (x:a -> PURE b (wpFun x)) = admit ()
+
+//  lem_wp_lambda'_monotonic wpCtx wpFun body fsG;
+//  reveal_opaque (`%pure_wp_monotonic) (pure_wp_monotonic u#b);
+// wp_lambda0' #g #a #b wpCtx wpFun body fsG
+
+
+unfold
+val helper_lambda' :
+  #g : env ->
+  #a : Type ->
+  #b : Type ->
+  wpCtx : spec_env (extend a g) b ->
+  wpFun : (a -> pure_wp b) ->
+  body : fs_oexp (extend a g) b wpCtx ->
+  fs_oexp g (x:a -> PURE b (wpFun x)) (wp_lambda' wpCtx wpFun body)
+let helper_lambda' wpCtx wpFun body fsG =
+  admit ();
+  fun x -> body (fs_stack fsG x)
+
+
+
+
 unfold
 val helper_refv: #g:env ->
                 #a:Type ->
@@ -226,10 +302,19 @@ type compilable : #a:Type -> g:env -> wp:spec_env g a -> fs_oexp g a wp -> Type 
                 #b :Type ->
                 #wpBody:spec_env (extend a g) b ->
                 #f :fs_oexp g (a -> b) (wp_lambda wpBody) ->
-                cf:compilable #b (extend a g)
-                              wpBody
-                              (helper_lambda f) ->
+                compilable #b (extend a g) wpBody (helper_lambda f) ->
                 compilable g (wp_lambda #g #a #b wpBody) f
+
+| QLambda :
+  #g : env ->
+  #a : Type ->
+  #b : Type ->
+  #wpCtx : spec_env (extend a g) b ->
+  #wpFun : (a -> pure_wp b) ->
+  #body : fs_oexp (extend a g) b wpCtx ->
+  compilable #b (extend a g) wpCtx body ->
+  compilable #(x:a -> PURE b (wpFun x)) g (wp_lambda' wpCtx wpFun body) (helper_lambda' wpCtx wpFun body)
+
 
 | CRefinement : #g:env ->
                 #a:Type ->
@@ -262,13 +347,7 @@ let test_app0 ()
 // FIXME, why does it need tactics to do such simple proofs?
 let test_app1 ()
   : Tot (compilable (extend (bool -> bool -> bool) empty) _ (fun fsG -> ((fs_hd fsG) true) false))
-  by (unfold_def (`wp_app);
-      explode ();
-       tadmit ();
-      trefl ();
-      trefl ();
-      trefl ()
-     )
+  by (dump "H")
   = CApp (CApp CVar0 CTrue) CFalse
 
 let test2_var
@@ -289,41 +368,41 @@ type compilable_debug #a (wp:spec_env empty a) (x:a) =
   compilable_closed #a #wp x
 
 let test1_exp ()
-  : compilable_closed #(bool -> bool) (fun x -> x)
-  = fun _ -> CLambda CVar0
+  : Tot (compilable_closed #(bool -> bool) (fun x -> x))
+  = fun _ -> QLambda CVar0
 
 let test1_exp' ()
   : Tot (compilable_closed #(bool -> bool -> bool) (fun x y -> y))
-  = fun _ ->  CLambda (CLambda CVar0)
+  = fun _ ->  QLambda (QLambda CVar0)
 
 let test_fapp1 ()
   : compilable_closed #((unit -> unit) -> unit) (fun f -> f ())
-  = fun _ -> CLambda (CApp CVar0 CUnit)
+  = fun _ -> QLambda (CApp CVar0 CUnit)
 
 let test_fapp2 ()
   : compilable_closed #((bool -> bool -> bool) -> bool) (fun f -> f true false)
-  = fun _ -> CLambda (CApp (CApp CVar0 CTrue) CFalse)
+  = fun _ -> QLambda (CApp (CApp CVar0 CTrue) CFalse)
 
 let test4_exp' ()
   : compilable_closed #(bool -> bool -> bool -> bool) (fun x y z -> x)
-  = fun _ -> CLambda (CLambda (CLambda CVar2))
+  = fun _ -> QLambda (QLambda (QLambda CVar2))
 
 let test5_exp' ()
   : compilable_closed #(bool -> bool -> bool -> bool) (fun x -> fun y z -> y)
-  = fun _ -> CLambda (CLambda (CLambda CVar1))
+  = fun _ -> QLambda (QLambda (QLambda CVar1))
 
 let test6_exp' ()
   : compilable_closed #(bool -> bool -> bool -> bool) (fun x y z -> z)
-  = fun _ -> CLambda (CLambda (CLambda CVar0))
+  = fun _ -> QLambda (QLambda (QLambda CVar0))
 
 [@expect_failure]
 let test4_exp'' ()
   : compilable_closed #(unit -> unit -> unit -> unit) (fun x y z -> y)
-  = fun _ -> CLambda (CLambda (CLambda CVar0))
+  = fun _ -> QLambda (QLambda (QLambda CVar0))
 
 let test1_hoc ()
   : compilable_closed #((bool -> bool) -> bool) (fun f -> f false)
-  = fun _ -> CLambda (CApp CVar0 CFalse)
+  = fun _ -> QLambda (CApp CVar0 CFalse)
 
 let test2_if0 ()
   : compilable_closed #(bool) (if true then false else true)
@@ -331,7 +410,7 @@ let test2_if0 ()
 
 let test2_if ()
   : compilable_closed #(bool -> bool) (fun x -> if x then false else true)
-  = fun _ -> CLambda (CIf CVar0 CFalse CTrue)
+  = fun _ -> QLambda (CIf CVar0 CFalse CTrue)
 
 #pop-options
 
@@ -352,86 +431,88 @@ let creame = (fun x -> if x then (fun y -> x) else (fun z -> z))
 
 let test3_if_ho ()
   : compilable_closed #(bool -> (bool -> bool)) creame
-  = fun _ -> CLambda (CIf CVar0
-                       (CLambda #_ #_ #_ #_ #myf CVar1) // TODO: why cannot it infer myf?
-                       (CLambda #_ #_ #_ #_ #myid CVar0))
+  by (dump "H")
+  = fun _ -> QLambda (CIf CVar0
+                       (QLambda CVar1) // TODO: why cannot it infer myf?
+                       (QLambda CVar0))
 
 let test1_if ()
   : compilable_closed #(bool -> bool -> bool) (fun x y -> if x then false else y)
-  = fun _ -> CLambda (CLambda (CIf CVar1 CFalse CVar0))
+  by (dump "H")
+  = fun _ -> QLambda (QLambda (CIf CVar1 CFalse CVar0))
 
 let test1_comp_ref ()
   : compilable_closed #(x:bool{x == true} -> x:bool{x == true}) (fun x -> x)
-  = fun _ -> CLambda CVar0
+  = fun _ -> QLambda CVar0
 
 let test1_erase_ref ()
   : compilable_closed #(x:bool{x == true} -> bool) (fun x -> x)
-  = fun _ -> CLambda (CRefinement _ CVar0)
+  = fun _ -> QLambda (CRefinement _ CVar0)
 
 open Examples
 
 let test_erase_refine_again ()
   : compilable_closed #(x:bool{p_ref x} -> x:bool{p_ref x}) (fun x -> x)
-  = fun _ -> CLambda (CRefinement _ (CRefinement _ CVar0))
+  = fun _ -> QLambda (CRefinement _ (CRefinement _ CVar0))
 
 [@expect_failure]
 let test_just_false
   : compilable_closed #(bool -> (x:bool{x == true})) (fun x -> false)
-  = fun _ -> CLambda (CRefinement _ CFalse)
+  = fun _ -> QLambda (CRefinement _ CFalse)
 
 let test_just_true' ()
   : compilable_closed just_true
-  = fun _ -> CLambda (CRefinement _ CTrue)
+  = fun _ -> QLambda (CRefinement _ CTrue)
 
 let test_moving_ref' ()
   : compilable_closed moving_ref
-  = fun _ -> CLambda (CRefinement _ CUnit)
+  = fun _ -> QLambda (CRefinement _ CUnit)
 
 let test_always_false' ()
   : compilable_closed always_false
-  = fun _ -> CLambda (CRefinement _ (CIf CVar0 (CFalse) CVar0))
+  by (dump "H")
+  = fun _ -> QLambda (CRefinement _ (CIf CVar0 (CFalse) CVar0))
 
 let test_always_false'' ()
   : Tot (compilable_closed always_false)
-  by (norm [delta_only [`%always_false]]) // TODO: why is the unfolding necessary?
+  by (norm [delta_only [`%always_false]]; dump "H") // TODO: why is the unfolding necessary?
   = fun _ ->
-    CLambda (CIf CVar0
+    QLambda (CIf CVar0
                 (CRefinement (fun y -> True) CFalse)
                 (CRefinement (fun y -> True) CVar0))
 
 let test_always_false_complex' ()
   : compilable_closed always_false_complex
-  = fun _ -> CLambda (CRefinement _ (CIf CVar0 (CIf CVar0 CFalse CTrue) CFalse))
+  = fun _ -> QLambda (CRefinement _ (CIf CVar0 (CIf CVar0 CFalse CTrue) CFalse))
 
 let test_always_false_complex'' ()
   : compilable_closed always_false_complex
-  = fun _ -> CLambda (CIf CVar0 (CIf CVar0 (CRefinement _ CFalse) (CRefinement _ CTrue)) (CRefinement _ CFalse))
+  = fun _ -> QLambda (CIf CVar0 (CIf CVar0 (CRefinement _ CFalse) (CRefinement _ CTrue)) (CRefinement _ CFalse))
 
 let test_always_false_ho ()
   : compilable_closed always_false_ho
-  = fun _ -> CLambda (CIf (CRefinement _ (CApp CVar0 CUnit)) (CRefinement _ CFalse) (CRefinement _ CTrue))
+  = fun _ -> QLambda (CIf (CRefinement _ (CApp CVar0 CUnit)) (CRefinement _ CFalse) (CRefinement _ CTrue))
 
 let test_if_x' ()
   : compilable_closed if_x
   by (norm [delta_only [`%if_x]]) // TODO: why is the unfolding necessary?
-  = fun _ -> CLambda (CLambda (CIf CVar0 (CApp CVar1 (CRefinement _ CVar0)) CFalse))
+  = fun _ -> QLambda (QLambda (CIf CVar0 (CApp CVar1 (CRefinement _ CVar0)) CFalse))
 
 let test_seq_basic' ()
-  : compilable_closed seq_basic
-  = fun _ -> CLambda (CSeq _ (CApp CVar0 CUnit) CUnit)
+  : compilable_closed (FStar.Pervasives.norm [delta_only [`%seq_basic]] seq_basic)
+  = fun _ -> QLambda (CSeq _ (CApp CVar0 CUnit) CUnit)
 
 let test_seq_qref' ()
   : compilable_closed seq_qref
-  = fun _ -> CLambda (CSeq _ (CApp CVar0 CUnit) (CRefinement _ CUnit))
+  = fun _ -> QLambda (CSeq _ (CApp CVar0 CUnit) (CRefinement _ CUnit))
 
 let test_seq_p_implies_q' ()
   : compilable_closed seq_p_implies_q
-  = fun _ -> CLambda (CLambda (CSeq _ (CApp CVar1 CVar0) (CRefinement _ CVar0)))
+  = fun _ -> QLambda (QLambda (CSeq _ (CApp CVar1 CVar0) (CRefinement _ CVar0)))
 
 let test_if_seq' ()
   : compilable_closed if_seq
-  by (norm [delta_only [`%if_seq]]) // TODO: why is the unfolding necessary?
-  = fun _ -> CLambda (CLambda (
+  = fun _ -> QLambda (QLambda (
      CIf CVar0
        (CSeq _ (CApp CVar1 (CRefinement _ CVar0))
                      (CRefinement _ CVar0))
@@ -446,10 +527,11 @@ let myid2 : fs_oexp (extend (f:(x:bool{x == true}) -> bool -> bool) (extend bool
 #push-options "--no_smt"
 
 let test_context' ()
-  : compilable_closed context
-  by (norm [delta_only [`%context]]; tadmit ()) // TODO: why is the unfolding necessary? // TODO: why is the tadmit necessary?
+  : compilable_closed (FStar.Pervasives.norm [delta_only [`%context];iota;unascribe] context)
+  by (dump "H")
+ // by (norm [delta_only [`%context]]; tadmit ()) // TODO: why is the unfolding necessary? // TODO: why is the tadmit necessary?
   = fun _ ->
     // TODO: why does it fail here?
-    CLambda (CLambda (CIf CVar1
+    QLambda (QLambda (CIf CVar1
                           (CApp CVar0 (CRefinement _ CVar1))
-                          (CLambda #_ #_ #_ #_ #(fun _ y -> y) CVar0)))
+                          (QLambda CVar0)))
